progress on the awkward example

theories/examples/awkward_example.v
@@ -10,13 +10,72 @@ Section awkward_example.
             MonRef: MonRefG (leibnizO _) CapR_rtc Σ,
             Heap: heapG Σ}.
 
+   Notation STS := (leibnizO (STS_states * STS_rels)).
+   Notation WORLD := (leibnizO (STS * STS)). 
+   Implicit Types W : WORLD.
+   
    (* choose a special register for the environment and adv pointer *)
    (* note that we are here simplifying the environment to simply point to one location *)      
    Definition r_env : RegName := r_t30.
-   Definition r_adv : RegName := r_t31.
+   Definition r_adv : RegName := r_t28.
    Definition r_self : RegName := r_t29.
-   
-   Ltac isWithinBounds := rewrite /withinBounds; apply andb_true_iff; split; apply Z.leb_le; simpl; auto.
+
+   (* Helper lemma to extract registers from a big_sepL2 *)
+   Lemma big_sepL2_extract_l {A B : Type} (i : nat) (ai : A) (a : list A) (b : list B) (φ : A -> B -> iProp Σ) :
+     a !! i = Some ai ->
+     (([∗ list] a_i;b_i ∈ a;b, φ a_i b_i) -∗
+     (∃ b', [∗ list] a_i;b_i ∈ (delete i a);b', φ a_i b_i) ∗ ∃ b, φ ai b)%I.
+   Proof. 
+     iIntros (Hsome) "Hl".
+     iDestruct (big_sepL2_length with "Hl") as %Hlength.      
+     assert (take i a ++ drop i a = a) as Heqa;[apply take_drop|]. 
+     assert (take i b ++ drop i b = b) as Heqb;[apply take_drop|]. 
+     rewrite -Heqa -Heqb.
+     iDestruct (big_sepL2_app_inv with "Hl") as "[Htake Hdrop]". 
+     { apply lookup_lt_Some in Hsome.
+       do 2 (rewrite take_length_le;[|lia]). done. 
+     }
+     apply take_drop_middle in Hsome as Hcons.
+     assert (ai :: drop (S i) a = drop i a) as Hh.
+     { apply app_inv_head with (take i a). congruence. }
+     rewrite -Hh.
+     iDestruct (big_sepL2_length with "Hdrop") as %Hlength'.      
+     destruct (drop i b);[inversion Hlength'|].
+     iDestruct "Hdrop" as "[Hφ Hdrop]".
+     iSplitR "Hφ";[|eauto].
+     iExists (take i b ++ l). rewrite Hcons. 
+     iDestruct (big_sepL2_app with "Htake Hdrop") as "Hl". 
+     rewrite delete_take_drop. iFrame.
+   Qed.
+
+   (* helper lemma to state that a fresh allocation creates a public future world *)
+   Lemma related_sts_pub_fresh (W : STS) a ρ i:
+    i ∉ dom (gset positive) W.1 →
+    i ∉ dom (gset positive) W.2 →
+    related_sts_pub W.1 (<[i:=a]> W.1) W.2 (<[i:=ρ]> W.2).
+  Proof.
+    intros Hdom_sta Hdom_rel.
+    rewrite /related_sts_pub. split;[|split;[auto|] ].
+    - apply dom_insert_subseteq.
+    - apply dom_insert_subseteq.
+    - apply not_elem_of_dom in Hdom_sta.
+      apply not_elem_of_dom in Hdom_rel.
+      intros j r1 r2 r1' r2' Hr Hr'.
+      destruct (decide (j = i)).
+      + subst. rewrite Hr in Hdom_rel. done.
+      + rewrite lookup_insert_ne in Hr'; auto.
+        rewrite Hr in Hr'. inversion Hr'. repeat (split;auto).
+        intros x y Hx Hy.
+        rewrite lookup_insert_ne in Hy;auto.
+        rewrite Hx in Hy.
+        inversion Hy; inversion Hr'; subst.
+        left.
+  Qed.
+     
+  Ltac isWithinBounds := rewrite /withinBounds; apply andb_true_iff; split; apply Z.leb_le; simpl; auto.
+
+  Ltac isWithinBounds_stack Hcont_stack index :=
+    isWithinBounds;[apply (incr_list_ge_middle _ index _ _ Hcont_stack);auto|apply (incr_list_le_middle _ index _ _ Hcont_stack);auto]. 
    
    Ltac iNotElemOfList :=
      repeat (apply not_elem_of_cons; split;[auto|]); apply not_elem_of_nil.  
@@ -41,14 +100,22 @@ Section awkward_example.
     iApply wp_pure_step_later;auto;iNext.
 
    Ltac iLookupR Hl :=
-    rewrite /= lookup_app_r;rewrite Hl /=;auto. 
+     rewrite /= lookup_app_r;rewrite Hl /=;auto.
+
+   Ltac iGet_genpur_reg Hr_gen Hwsr wsr ptr :=
+     let w := fresh "wr" in 
+     destruct wsr as [? | w wsr]; first (by inversion Hwsr);
+     iDestruct Hr_gen as ptr.
+
+   Ltac iCorrectPC a_first a a_last index Hcont :=
+     apply isCorrectPC_bounds_alt with a_first a_last;auto;iContiguous_bounds a_first a a_last index Hcont.
     
    (* Recall that the malloc subroutine lies in b_m e_m *)
 
    (* assume that r1 contains an executable pointer to the malloc subroutine *)
    Definition awkward_preamble_instrs r1 offset_to_awkward :=
      [move_r r_t0 PC;
-     lea_z r_self 1;
+     lea_z r_t0 3;
      jmp r1;
      move_r r_self PC;
      lea_z r_self offset_to_awkward;
@@ -102,11 +169,23 @@ Section awkward_example.
    Definition awk_inv i a :=
      (∃ x:bool, sts_state_loc i x
            ∗ if x
-             then a ↦ₐ[RW] inl 1%Z
-             else a ↦ₐ[RW] inl 0%Z)%I.
+             then a ↦ₐ[RWX] inl 1%Z
+             else a ↦ₐ[RWX] inl 0%Z)%I.
 
    Definition awk_rel_pub := λ a b, a = false ∨ b = true.
    Definition awk_rel_priv := λ (a b : bool), True.
+
+   Inductive local_state :=
+   | First
+   | Second
+   | Released. 
+   Definition local_rel_pub := λ (a b : local_state), a = b.
+   Definition local_rel_priv := λ (a b : local_state), (a = First ∧ b = Second) ∨ (a = Second ∧ b = Released). 
+
+   Definition awk_W W i : WORLD := (W.1,(<[i:=countable.encode false]>W.2.1,<[i:=(convert_rel awk_rel_pub,convert_rel awk_rel_priv)]>W.2.2)).
+
+   (* namespace definitions for the regions *)
+   Definition regN : namespace := nroot .@ "regN".
 
    (* the following spec is for the preamble to the awkward example. It allocates the invariant on the malloc'ed region *)
    Lemma g1_spec φ W pc_p pc_g pc_b pc_e (* PC *)
@@ -124,24 +203,145 @@ Section awkward_example.
      (* Address assumptions *)
      (a_first + (3 + offset_to_awkward))%a = Some a_cont ->
 
-     (PC ↦ᵣ inr ((pc_p,pc_g),pc_b,pc_e,a_first)
+     ((* PC *)
+       PC ↦ᵣ inr ((pc_p,pc_g),pc_b,pc_e,a_first)
+      (* assume r_t1 points to a the malloc subroutine *)
       ∗ r_t1 ↦ᵣ inr (E,Global,b_m,e_m,a_m)
-      ∗ (∃ wsr, [∗ list] r_i;w_i ∈ list_difference all_registers [PC;r_t1]; wsr, r_i ↦ᵣ w_i)
+      ∗ [[b_m,e_m]] ↦ₐ[p_m] [[malloc_subroutine r_env 1]]
+      (* general purpose registers *)
+      ∗ (∃ wsr, [∗ list] r_i;w_i ∈ list_difference all_registers [r_t1;PC]; wsr, r_i ↦ᵣ w_i)
+      (* program *)
       ∗ awkward_preamble g1_addrs pc_p r_t1 offset_to_awkward
+      (* region invariants *)
       ∗ region W
       ∗ sts_full_world sts_std W
-      ∗ ▷ (PC ↦ᵣ inr ((pc_p,pc_g),pc_b,pc_e,a_cont)
+      (* continuation *)
+      ∗ ▷ ((PC ↦ᵣ inr ((pc_p,pc_g),pc_b,pc_e,a_cont)
           ∗ r_self ↦ᵣ inr ((pc_p,pc_g),pc_b,pc_e,a_cont)
-          ∗ (∃ wsr, [∗ list] r_i;w_i ∈ list_difference all_registers [PC;r_self]; wsr, r_i ↦ᵣ w_i)
+          ∗ (∃ wsr, [∗ list] r_i;w_i ∈ list_difference all_registers [PC;r_self;r_env]; wsr, r_i ↦ᵣ w_i)    
+          ∗ ∃ d, r_env ↦ᵣ inr (RWX,Global,d,d,d)
+          ∗ (∃ (i : positive), region (awk_W W i) ∗ sts_full_world sts_std (awk_W W i) ∗ sts_rel_loc i awk_rel_pub awk_rel_priv ∗ (∃ ι, inv ι (awk_inv i d))))
           -∗ WP Seq (Instr Executable) {{ φ }})
       ⊢ WP Seq (Instr Executable) {{ φ }})%I.
-     
+   Proof. 
+     iIntros ([Hvpc1 Hvpc2] Hcont [Hfirst Hlast] Ha_cont) "(HPC & Hr_t1 & Hmalloc & Hr_gen & Hprog & Hr & Hsts & Hφ)".
+     iDestruct (big_sepL2_length with "Hprog") as %Hprog_length.
+     destruct g1_addrs; [inversion Hprog_length|].
+     simpl in Hfirst; inversion Hfirst; subst.
+     iDestruct "Hr_gen" as (wsr) "Hr_gen".
+     iDestruct (big_sepL2_length with "Hr_gen") as %Hwsr.
+     rewrite /all_registers /=. 
+     iGet_genpur_reg "Hr_gen" Hwsr wsr "[Hr_t0 Hr_gen]". 
+     (* move r_t1 PC *)
+     iPrologue g1_addrs Hprog_length "Hprog".
+     iApply (wp_move_success_reg_fromPC with "[$HPC $Hinstr $Hr_t0]");
+       [apply move_r_i|apply PermFlows_refl|auto|iContiguous_next Hcont 0|auto|].
+     iEpilogue "(HPC & Hprog_done & Hr_t0)".
+     (* lea r_t0 2 *)
+     iPrologue g1_addrs Hprog_length "Hprog".
+     destruct g1_addrs;[inversion Hprog_length|].
+     assert (a_first + 3 = Some a1)%a as Ha1;[apply (contiguous_incr_addr _ 3 a_first _ Hcont); auto|].
+     iApply (wp_lea_success_z with "[$HPC $Hinstr $Hr_t0]");
+       [apply lea_z_i|apply PermFlows_refl|iCorrectPC a_first a a_last 1 Hcont|iContiguous_next Hcont 1|apply Ha1|auto..]. 
+     { destruct pc_p; auto. inversion Hvpc1 as [?????? [Hcontr | [Hcontr | Hcontr] ] ];inversion Hcontr. }
+     iEpilogue "(HPC & Ha & Hr_t0)". iCombine "Ha" "Hprog_done" as "Hprog_done". 
+     (* jmp r_t1 *)
+     iPrologue g1_addrs Hprog_length "Hprog". 
+     iApply (wp_jmp_success with "[$HPC $Hinstr $Hr_t1]");
+       [apply jmp_i|apply PermFlows_refl|iCorrectPC a_first a0 a_last 2 Hcont|]. 
+     iEpilogue "(HPC & Ha0 & Hr_t1)"; iCombine "Ha0" "Hprog_done" as "Hprog_done".
+     iSimpl in "HPC". 
+     (* malloc subroutine *)
+     iApply (malloc_spec W); last iFrame "Hmalloc Hr_t0 HPC".
+     iSplitL "Hr_gen Hr_t1".
+     { iExists (_ :: wsr). rewrite /all_registers /=. iFrame. }
+     iNext. iIntros "(_ & Hgen_reg & HPC & Hbe)".
+     (* Since we are dynamically allocating local state, we do not need the freshness requirement *)
+     iDestruct "Hbe" as (b e Hsize) "(Hr_env & Hbe & _)".
+     (* Allocate a new invariant *)
+     rewrite Z.sub_diag in Hsize. rewrite /region_mapsto /region_addrs_zeroes /region_addrs. 
+     destruct (Z_le_dec b e);[|omega]. 
+     assert (region_size b e = 1) as ->;[by rewrite /region_size Hsize /=|]. 
+     iDestruct "Hbe" as "[Hb _]".
+     iDestruct "Hgen_reg" as (wsr') "Hgen_reg". clear Hwsr. 
+     iMod (sts_alloc_loc W false awk_rel_pub awk_rel_priv with "Hsts")
+       as (i) "(Hsts & % & % & Hstate & #Hrel)".
+     iMod (inv_alloc (regN.@b) _ (awk_inv i b) with "[Hstate Hb]")%I as "#Hb".
+     { iNext. iExists false. iFrame. }
+     (* Prepare to jump to f4 *)
+     (* move_r r_self PC *)
+     iDestruct "Hprog" as "[Hinstr Hprog]".
+     iApply (wp_bind (fill [SeqCtx])).
+     iDestruct (big_sepL2_extract_l 29 r_self with "Hgen_reg") as "[Hr_gen Hr_self]";[auto|rewrite /all_registers /=].
+     iDestruct "Hr_self" as (w) "Hr_self". 
+     iApply (wp_move_success_reg_fromPC with "[$HPC $Hinstr $Hr_self]");
+       [apply move_r_i|apply PermFlows_refl|iCorrectPC a_first a1 a_last 3 Hcont|iContiguous_next Hcont 3|auto|]. 
+     iEpilogue "(HPC & Hinstr & Hr_self)"; iCombine "Hinstr" "Hprog_done" as "Hprog_done".
+     (* lea r_self offset_to_awkward *)
+     iPrologue g1_addrs Hprog_length "Hprog".
+     assert ((a1 + offset_to_awkward)%a = Some a_cont) as Hcont';[rewrite (addr_add_assoc _ a1) in Ha_cont;auto|].
+     iApply (wp_lea_success_z with "[$HPC $Hinstr $Hr_self]");
+       [apply lea_z_i|apply PermFlows_refl|iCorrectPC a_first a2 a_last 4 Hcont|iContiguous_next Hcont 4|apply Hcont'|auto..].
+     { destruct pc_p; auto. inversion Hvpc1 as [?????? [Hcontr | [Hcontr | Hcontr] ] ];inversion Hcontr. }
+     iEpilogue "(HPC & Hinstr & Hr_self)"; iCombine "Hinstr" "Hprog_done" as "Hprog_done".
+     (* jmp r_self *)
+     iDestruct "Hprog" as "[Hinstr _]".
+     iApply (wp_bind (fill [SeqCtx])).
+     iApply (wp_jmp_success with "[$HPC $Hinstr $Hr_self]");
+       [apply jmp_i|apply PermFlows_refl|iCorrectPC a_first a3 a_last 5 Hcont|].
+     iEpilogue "(HPC & Hinstr & Hr_self)"; iCombine "Hinstr" "Hprog_done" as "_".
+     (* continuation *)
+     iApply "Hφ". iFrame "Hr_gen Hr_self".
+     iSplitL "HPC".
+     { destruct pc_p; iFrame. inversion Hvpc1 as [?????? [Hcontr | [Hcontr | Hcontr] ] ];inversion Hcontr. }
+     assert (b = e)%a as ->;[apply z_of_eq;lia|].
+     iExists e. iFrame.
+     iExists i. iFrame "∗ #". iSplitL;[|eauto]. 
+     iApply (region_monotone with "[] [] Hr"); [auto|].
+     iPureIntro. split;[apply related_sts_pub_refl|simpl]. 
+     apply related_sts_pub_fresh; auto.
+   Qed.
+
+   Import uPred.
+
+   (* TODO: move this to separate region lemma file *)
+   Lemma monotone_revoked_close_sub' W l p φ :
+    ([∗ list] a ∈ l, temp_resources W φ a p ∗ rel a p φ ∗ ⌜revoked W a⌝)
+    ∗ sts_full_world sts_std W ∗ region W ==∗
+    sts_full_world sts_std (close_list (countable.encode <$> l) W)
+    ∗ region (close_list (countable.encode <$> l) W).
+  Admitted. 
    
+
+
+   (* The proof of the awkward example goes through a number of worlds.
+      Below are some helper lemmas and definitions about how these worlds 
+      are related *)
+   Lemma related_priv_local_1 W i :
+     W.2.1 !! i = Some (countable.encode true) ->
+     W.2.2 !! i = Some (convert_rel awk_rel_pub, convert_rel awk_rel_priv) ->
+     related_sts_priv_world W (W.1, (<[i:=countable.encode false]> W.2.1, W.2.2)).
+   Proof.
+     intros Hlookup Hrel. 
+     split;[apply related_sts_priv_refl|simpl].
+     split;[apply dom_insert_subseteq|split;[auto|] ].
+     intros j r1 r2 r1' r2' Hr Hr'.
+     rewrite Hr in Hr'. inversion Hr'; subst; repeat (split;auto).
+     intros x y Hx Hy.
+     destruct (decide (i = j)).
+     - subst. rewrite lookup_insert in Hy; inversion Hy; subst.
+       rewrite Hrel in Hr. rewrite Hlookup in Hx. inversion Hr; inversion Hx; subst.
+       right with (countable.encode false);[|left].
+       right. exists true,false. repeat (split;auto).
+     - rewrite lookup_insert_ne in Hy;auto. rewrite Hx in Hy; inversion Hy; subst. left.
+   Qed. 
+   
+     
    (* the following spec is for the f4 subroutine of the awkward example, jumped to after dynamically allocating into r_env *)
    Lemma f4_spec W pc_p pc_g pc_b pc_e (* PC *)
          b e a (* adv *)
          f4_addrs flag_off (* f2 *)
-         d d' i (* dynamically allocated memory given by preamble, connected to invariant i *)
+         d i (* dynamically allocated memory given by preamble, connected to invariant i *)
          a_first a_last a_flag (* special adresses *) 
          (b_r e_r b_r' : Addr) (* stack *) :
     
@@ -159,9 +359,6 @@ Section awkward_example.
      region_size b_r e_r > 12 -> (* we must assume the stack is large enough for needed local state *)
      (b_r' + 1)%a = Some b_r ->
 
-     (* Preamble assumptions *)
-     (d + 1)%a = Some d' ->
-
      (* Finally, we must assume that the stack is currently in a revoked state *)
      Forall (λ a, revoked W a ∧ rel_is_std_i W (countable.encode a)) (region_addrs b_r e_r) ->
 
@@ -169,19 +366,20 @@ Section awkward_example.
       ∗ PC ↦ᵣ inr ((pc_p,pc_g),pc_b,pc_e,a_first)
       ∗ r_self ↦ᵣ inr ((pc_p,pc_g),pc_b,pc_e,a_first)
       ∗ r_adv ↦ᵣ inr ((E,Global),b,e,a)
-      ∗ r_env ↦ᵣ inr (RWX,Global,d,d',d)
+      ∗ r_env ↦ᵣ inr (RWX,Global,d,d,d)
       ∗ (∃ wsr, [∗ list] r_i;w_i ∈ list_difference all_registers [PC;r_stk;r_adv;r_self;r_env]; wsr, r_i ↦ᵣ w_i)
       (* invariant for d *)
-      ∗ awk_inv i d
+      ∗ (∃ ι, inv ι (awk_inv i d))
       ∗ sts_rel_loc i awk_rel_pub awk_rel_priv
       (* stack *)
       ∗ (∃ ws, [[b_r, e_r]]↦ₐ[RWLX][[ws]])
+      ∗ ([∗ list] a ∈ (region_addrs b_r e_r), rel a RWLX (λ Wv : prodO STS STS * Word, (interp Wv.1) Wv.2))
       (* flag *)
       ∗ a_flag ↦ₐ[RW] inl 0%Z
       (* token which states all non atomic invariants are closed *)
       ∗ na_own logrel_nais ⊤
       (* adv code *)
-      ∗ interp W (inr ((E,Global),b,e,a))
+      ∗ ([∗ list] a ∈ (region_addrs b e), (read_write_cond a RX interp) ∧ ⌜region_state_nwl W a Global⌝ ∧ ⌜region_std W a⌝)
       (* trusted code *)
       ∗ awkward_example f4_addrs pc_p r_self r_adv 65 flag_off
       (* we start out with arbitrary sts *)
@@ -191,8 +389,259 @@ Section awkward_example.
       Seq (Instr Executable)
     {{{ v, RET v; ⌜v = HaltedV⌝ → a_flag ↦ₐ[RW] inl 0%Z }}}.
   Proof.
-                
-
-   
-
+    iIntros ([Hvpc1 Hvpc2] Hcont [Hfirst Hlast] Hpos Hle Hl_bound Hb_r Hrevoked φ)
+            "(Hr_stk & HPC & Hr_self & Hr_adv & Hr_env & Hgen_reg & #Hι & #Hrel & Hstack & #Hstack_val & Hflag & Hna & Hadv_val & Hprog & Hsts & Hr) Hφ".
+    (* We put the code in a non atomic invariant for each iteration of the program *)
+    iMod (na_inv_alloc logrel_nais ⊤ (nroot.@"prog") with "Hprog") as "#Hf4". 
+    (* Since the program will jump to itself, we need to do a Lob induction *)
+    (* We generalize the induction over all W *)
+    iRevert (Hrevoked). iLöb as "IH" forall (W).
+    iIntros (Hrevoked).
+    (* Now we step through the iteration *)
+    iMod (na_inv_open with "Hf4 Hna") as "(>Hprog & Hna & Hcls)";[auto..|]. 
+    iDestruct (big_sepL2_length with "Hprog") as %Hprog_length.
+    destruct (f4_addrs);[inversion Hprog_length|].
+    iDestruct "Hι" as (ι) "Hinv". 
+    (* We will now need to open the invariant for d. 
+       We do not know which state d is in, and may need to 
+       do a private transition from 1 to 0! For that reason 
+       we will first revoke region, so that we can do private 
+       updates to it. We do not care about the stack resources, 
+       as it currently in the revoked state. 
+     *)
+    iMod (monotone_revoke with "[$Hsts $Hr]") as "[Hsts Hr]". 
+    (* Now we may do any private transitions to our local invariants.
+       since we don't know which case we are in, we can generalize and 
+       say that there exists some private future world such that   
+       the store succeeded, after which the state at i is false
+     *)
+    iPrologue l Hprog_length "Hprog".
+    simpl in Hfirst. inversion Hfirst; subst. 
+    iAssert (▷ (PC ↦ᵣ inr (pc_p, pc_g, pc_b, pc_e, a1)
+              ∗ r_env ↦ᵣ inr (RWX, Global, d, d, d)
+              ∗ a_first ↦ₐ[pc_p] store_z r_env 0
+              ∗ (∃ W', ⌜related_sts_priv_world (revoke W) W'⌝ ∧
+                       ⌜W'.2.1 !! i = Some (countable.encode false)⌝ ∧
+                       region W' ∗ sts_full_world sts_std W' ∗
+                       ⌜Forall (λ a : Addr, revoked W' a ∧ rel_is_std_i W' (countable.encode a)) (region_addrs b_r e_r)⌝)
+              -∗ WP Seq (Instr Executable) {{ v, φ v }})
+        -∗ WP Instr Executable {{ v, WP fill [SeqCtx] (of_val v) {{ v, φ v }} }})%I
+      with "[HPC Hinstr Hr_env Hr Hsts]" as "Hstore_step".
+    { iIntros "Hcont". 
+      (* store r_env 0 *)
+      iInv ι as (x) "[>Hstate Hb]" "Hcls".
+      destruct x; iDestruct "Hb" as ">Hb".
+      - iApply (wp_store_success_z with "[$HPC $Hinstr $Hr_env $Hb]");
+          [apply store_z_i|apply PermFlows_refl|apply PermFlows_refl|auto|iContiguous_next Hcont 0| |auto|..].
+        { split;auto. isWithinBounds; lia. }
+        iNext. iIntros "(HPC & Hinstr & Hr_env & Hd)".
+        (* we assert that updating the local state d to 0 is a private transition *)
+        iDestruct (sts_full_state_loc with "Hsts Hstate") as %Hlookup.
+        iDestruct (sts_full_rel_loc with "Hsts Hrel") as %Hrel.
+        assert (related_sts_priv_world W (W.1, (<[i:=countable.encode false]> W.2.1, W.2.2)))
+          as Hrelated;[apply related_priv_local_1; auto|].
+        (* first we can update region privately since it is revoked *)
+        iAssert (sts_full_world sts_std (revoke W)
+               ∗ region ((revoke W).1, (<[i:=countable.encode false]> (revoke W).2.1, (revoke W).2.2)))%I with "[Hsts Hr]" as "[Hsts Hr]".
+        { rewrite region_eq /region_def.
+          iDestruct "Hr" as (M) "(HM & % & Hr)".
+          iDestruct (monotone_revoke_list_region_def_mono $! Hrelated with "[] Hsts Hr") as "[Hsts Hr]".
+          - iPureIntro. by apply dom_equal_revoke.
+          - iFrame. iExists M. iFrame. iPureIntro. auto.
+        }
+        (* we must update the local state of d to false *)
+        iMod (sts_update_loc _ _ _ false with "Hsts Hstate") as "[Hsts Hstate]". 
+        iMod ("Hcls" with "[Hstate Hd]") as "_". 
+        { iNext. iExists false. iFrame. }
+        iModIntro. iApply wp_pure_step_later;auto;iNext.
+        iApply "Hcont". iFrame "HPC Hr_env Hinstr".
+        iExists _.
+        iDestruct (sts_full_world_std with "[] Hsts") as %Hstd; [iPureIntro;split;apply related_sts_priv_refl|].
+        iFrame "Hsts Hr". iSimpl.
+        iPureIntro. split;[apply revoke_monotone in Hrelated; auto|split;[apply lookup_insert|] ].
+        eapply Forall_impl;[|apply Hrevoked].
+        intros a0 [Ha0_rev Ha0_std]. split;auto. 
+        rewrite /revoked /std_sta /=. rewrite /revoked /= in Ha0_rev.
+        destruct (W.1.1 !! countable.encode a0) eqn:Hsome;[subst|done].
+        apply revoke_lookup_Revoked in Hsome. rewrite Hsome. done. 
+      - iApply (wp_store_success_z with "[$HPC $Hinstr $Hr_env $Hb]");
+          [apply store_z_i|apply PermFlows_refl|apply PermFlows_refl|auto|iContiguous_next Hcont 0| |auto|..].
+        { split;auto. isWithinBounds; lia. }
+        iNext. iIntros "(HPC & Hinstr & Hr_env & Hd)".
+        (* use sts_state to assert that the current state of i is false *)
+        iDestruct (sts_full_state_loc with "Hsts Hstate") as %Hlookup. 
+        (* No need to update the world, since we did not change state *)
+        iMod ("Hcls" with "[Hstate Hd]") as "_". 
+        { iNext. iExists false. iFrame. }
+        iModIntro. iApply wp_pure_step_later;auto;iNext.
+        iApply "Hcont". iFrame "HPC Hr_env Hinstr".
+        iExists _. iFrame. iPureIntro. split;[split;apply related_sts_priv_refl|split;auto].
+        eapply Forall_impl;[|apply Hrevoked].
+        intros a0 [Ha0_rev Ha0_std]. split;auto. 
+        rewrite /revoked /std_sta /=. rewrite /revoked /= in Ha0_rev.
+        destruct (W.1.1 !! countable.encode a0) eqn:Hsome;[subst|done].
+        apply revoke_lookup_Revoked in Hsome. rewrite Hsome. done. 
+    }
+    iApply "Hstore_step". 
+    iNext. iIntros "(HPC & Hr_env & Hprog_done & HW')".
+    iDestruct "HW'" as (W' Hrelated Hfalse) "(Hr & Hsts & #Hforall)".
+    clear Hrevoked. iDestruct "Hforall" as %Hrevoked. 
+    (* we prepare the stack for storing local state *)
+    iDestruct "Hstack" as (ws) "Hstack".
+    iDestruct (big_sepL2_length with "Hstack") as %Hstack_length.
+    assert (∃ ws_local ws_rest, ws = ws_local ++ ws_rest ∧ length ws_local = 3)
+      as [ws_local [ws_rest [Happ Hlocal_length] ] ].
+    { rewrite region_addrs_length in Hstack_length; auto. rewrite Hstack_length in Hl_bound. 
+      do 3 (destruct ws as [|? ws]; [simpl in Hl_bound; lia|]). by exists [w;w0;w1],ws. }
+    rewrite Happ.
+    iDestruct (contiguous_program_split with "Hstack") as (stack_local stack_rest s_last s_first)
+                                                            "(Hstack_local & Hstack_rest & #Hcont)";
+      [apply region_addrs_contiguous|lia|..].
+    { rewrite Happ region_addrs_length in Hstack_length;[|auto]. rewrite app_length in Hstack_length. lia. }
+    iDestruct "Hcont" as %(Hstack_local & Hstack_rest & Hstackeq & Hs_last & Hs_first & Hlink).
+    iDestruct (big_sepL2_length with "Hstack_local") as %Hlength_local. rewrite Hlocal_length in Hlength_local. 
+    do 3 (destruct stack_local;[inversion Hlength_local|]). destruct stack_local;[|inversion Hlength_local]. 
+    do 3 (destruct ws_local;[inversion Hlocal_length|]). destruct ws_local;[|inversion Hlocal_length]. 
+    assert (a0 = b_r) as Heq;[|simplify_eq]. 
+    { assert (region_addrs b_r e_r !! 0 = Some b_r) as Hfirst';[apply region_addrs_first;auto|].
+      rewrite Hstackeq /= in Hfirst'. inversion Hfirst'; done. 
+    }
+    iDestruct "Hstack_local" as "(Hb_r & Ha2 & Ha3 & _)".
+    assert (contiguous (region_addrs b_r e_r)) as Hcont_stack;[apply region_addrs_contiguous|].
+    assert (list.last ([b_r; a2; a3] ++ stack_rest) = Some e_r) as Hlast_stack.
+    { rewrite -Hstackeq. apply region_addrs_last;auto. }
+    rewrite Hstackeq in Hcont_stack.
+    (* push r_stk r_env *)
+    do 2 (destruct l;[inversion Hprog_length|]).
+    iDestruct (big_sepL2_app_inv _ [a1;a0] (a4::l) with "Hprog") as "[Hpush Hprog]";[simpl;auto|]. 
+    iApply (push_r_spec);[..|iFrame "HPC Hr_stk Hpush Hr_env Hb_r"];
+      [|apply PermFlows_refl|by isWithinBounds|iContiguous_next Hcont 1|iContiguous_next Hcont 2|apply Hb_r|..].
+    { split;[iCorrectPC a_first a1 a_last 1 Hcont|iCorrectPC a_first a0 a_last 2 Hcont]. }
+    iNext. iIntros "(HPC & Hpush & Hr_stk & Hr_env & Hb_r)". iCombine "Hpush" "Hprog_done" as "Hprog_done".
+    (* push r_stk r_self *)
+    do 2 (destruct l;[inversion Hprog_length|]).
+    iDestruct (big_sepL2_app_inv _ [a4;a5] (a6::l) with "Hprog") as "[Hpush Hprog]";[simpl;auto|]. 
+    iApply (push_r_spec);[..|iFrame "HPC Hr_stk Hpush Hr_self Ha2"];
+      [|apply PermFlows_refl|isWithinBounds_stack Hcont_stack 1|iContiguous_next Hcont 3|
+       iContiguous_next Hcont 4|iContiguous_next Hstack_local 0|..].
+    { split;[iCorrectPC a_first a4 a_last 3 Hcont|iCorrectPC a_first a5 a_last 4 Hcont]. }
+    iNext. iIntros "(HPC & Hpush & Hr_stk & Hr_self & Ha2)". iCombine "Hpush" "Hprog_done" as "Hprog_done".
+    (* push r_stk r_adv *)
+    do 2 (destruct l;[inversion Hprog_length|]).
+    iDestruct (big_sepL2_app_inv _ [a6;a7] (a8::l) with "Hprog") as "[Hpush Hprog]";[simpl;auto|]. 
+    iApply (push_r_spec);[..|iFrame "HPC Hr_stk Hpush Hr_adv Ha3"];
+      [|apply PermFlows_refl|isWithinBounds_stack Hcont_stack 2|iContiguous_next Hcont 5|
+       iContiguous_next Hcont 6|iContiguous_next Hstack_local 1|..].
+    { split;[iCorrectPC a_first a6 a_last 5 Hcont|iCorrectPC a_first a7 a_last 6 Hcont]. }
+    iNext. iIntros "(HPC & Hpush & Hr_stk & Hr_adv & Ha3)". iCombine "Hpush" "Hprog_done" as "Hprog_done".
+    
+    (* need to split the stack in additionally two parts: own and adv *)
+    iDestruct (big_sepL2_length with "Hstack_rest") as %Hlength_stack_rest.
+     assert (∃ ws_own ws_adv, ws_rest = ws_own ++ ws_adv ∧ length ws_own = 8)
+      as [ws_own [ws_adv [Happ Hlength'] ] ].
+    { rewrite region_addrs_length in Hstack_length; auto. rewrite Hstack_length in Hl_bound. 
+      do 8 (destruct ws_rest as [|? ws_rest]; [simpl in Hl_bound; lia|]).
+           by exists [w2;w3;w4;w5;w6;w7;w8;w9],ws_rest. }
+    rewrite Happ.
+    iDestruct (contiguous_program_split with "Hstack_rest") as (stack_own stack_adv s_last' s_first')
+                                                            "(Hstack_own & Hstack_adv & #Hcont)";
+      [repeat (apply contiguous_weak in Hcont_stack;try done)|lia|..].
+    { rewrite Happ region_addrs_length in Hstack_length;[|auto]. do 2 (rewrite app_length in Hstack_length). lia. }
+    iDestruct "Hcont" as %(Hstack_own & Hstack_adv & Hstackeq' & Hs_last' & Hs_first' & Hlink'').
+    assert (contiguous (region_addrs b_r e_r)) as Hstackcont;[apply region_addrs_contiguous|rewrite Hstackeq in Hstackcont]. 
+    iDestruct (big_sepL2_length with "Hstack_own") as %Hlength_own. rewrite Hlength' in Hlength_own.
+    (* prepare for scall *)
+    (* split the program into the scall_prologue and the rest *)
+    iDestruct (contiguous_program_split with "Hprog") as (scall_prologue rest0 scall_last rest0_first)
+                                                         "(Hscall & Hf2 & #Hcont)"; [auto|simpl;lia|simpl;lia|..].
+    { repeat (apply contiguous_weak in Hcont; try done). }
+    iDestruct "Hcont" as %(Hcont_scall & Hcont_rest0 & Hrest_app & Hscall_last & Hrest0_first & Hlink'). subst.
+    iDestruct (big_sepL2_length with "Hscall") as %Hscall_length. simpl in Hscall_length.
+    destruct scall_prologue as [|scall_prologue_first scall_prologue];[inversion Hscall_length|].
+    assert (scall_prologue_first = a8) as <-;[inversion Hrest_app;auto|].
+    (* get important elements of the stack *)
+    destruct stack_own as [|stack_own_b stack_own];[inversion Hlength_own|].
+    assert ((stack_own_b :: stack_own) = region_addrs stack_own_b s_last') as ->.
+    { apply contiguous_region_addrs; auto. }
+    assert (stack_adv = region_addrs s_first' e_r) as ->.
+    { apply contiguous_region_addrs; auto. rewrite -(region_addrs_last b_r);[|auto].
+      rewrite Hstackeq. rewrite -last_app_eq; [auto|simpl;lia]. rewrite -last_app_eq;[auto|]. destruct stack_adv; [inversion Hs_first'|simpl;lia]. }
+    assert ((stack_own_b + 7)%a = Some s_last') as Hstack_own_bound.
+    { apply (contiguous_incr_addr_middle _ 0 7 stack_own_b _ Hstack_own); auto. simpl.
+      assert (length stack_own - 1 = 6) as Heq;[simpl in Hlength_own;lia|]. rewrite -Heq. 
+      rewrite -last_lookup. simpl in Hs_last. destruct stack_own; [inversion Heq|done]. }
+    (* Scall *)
+    iApply scall_prologue_spec; last (iFrame "Hscall HPC Hr_stk"; iSplitL "Hgen_reg Hr_env Hr_self";
+                                      [|iSplitL "Hstack_own";[iNext;eauto|iSplitL "Hstack_adv";[iNext;eauto|] ] ]);
+      [iCorrectPC a_first scall_prologue_first a_last 7 Hcont| |isWithinBounds_stack Hcont_stack 3| |apply Hpos|apply Hcont_scall|auto|apply Hscall_last|
+       apply PermFlows_refl|iNotElemOfList|iContiguous_next Hstackcont 2|apply Hstack_own_bound|..|apply Hlink'| |].
+    { assert (length scall_prologue - 1 = 75) as Heq;[simpl in Hscall_length; lia|]. 
+      iCorrectPC a_first scall_last a_last 83 Hcont;
+      (rewrite Hrest_app /= lookup_app_l;[rewrite -Heq -last_lookup; destruct scall_prologue;[inversion Hscall_length|auto]|simpl in Hscall_length;lia]). }
+    { isWithinBounds_stack Hstackcont 11; inversion Hlength_own as [Heq]; rewrite /= Heq lookup_app_r;rewrite Heq; auto. }
+    { assert (8 = 7 + 1)%Z as ->;[auto|]. rewrite (addr_add_assoc _ s_last'); auto. }
+    { apply (contiguous_incr_addr_middle _ 7 77 scall_prologue_first _ Hcont); auto.
+      rewrite -Hscall_length Hrest_app /= lookup_app_r;[|lia]. rewrite PeanoNat.Nat.sub_diag; auto. }
+    { iNext. iDestruct "Hgen_reg" as (wsr) "Hgen_reg". iExists (wsr ++ [_;_]). rewrite /all_registers /=.
+      iApply (big_sepL2_app _ _ [r_t29; r_t30] wsr with "Hgen_reg [Hr_env Hr_self]").
+      by iFrame. }
+    iNext. iIntros "(HPC & Hr_stk & Hr_t0 & Hgen_reg & Hstack_own & Hstack_adv & Hscall)".
+    iCombine "Hscall" "Hprog_done" as "Hprog_done".
+    assert (isCorrectPC (inr (pc_p, pc_g, pc_b, pc_e, rest0_first))) as Hvpc1'.
+    { iCorrectPC a_first rest0_first a_last 84 Hcont;
+      (rewrite Hrest_app /=;inversion Hscall_length; rewrite lookup_app_r;[rewrite PeanoNat.Nat.sub_diag; auto|auto]). }
+    (* jmp r_adv *)
+    iDestruct (big_sepL2_length with "Hf2") as %Hrest_length; simpl in Hrest_length. 
+    destruct rest0;[inversion Hrest_length|]. 
+    iPrologue rest0 Hrest_length "Hf2". inversion Hrest0_first; subst.
+    iApply (wp_jmp_success with "[$Hinstr $Hr_adv $HPC]");
+      [apply jmp_i|apply PermFlows_refl|auto|..].
+    iEpilogue "(HPC & Hinstr & Hr_adv)". iSimpl in "HPC".
+    (* We now want to reason about unknows code. For this we invoke the fundamental theorem *)
+    (* Before we can show the validity of the continuation, we need to set up the invariants 
+       for local state, as well as the invariant for the stack *)
+    (* We start out by closing the invariant for the program *)
+    iMod ("Hcls" with "[Hprog_done Hinstr Hprog $Hna]") as "Hna". 
+    { iNext. iDestruct "Hprog_done" as "(Hscall & Hpush3 & Hpush2 & Hpush1 & Ha_first)".
+      iFrame "Ha_first". rewrite Hrest_app. 
+      iApply (big_sepL2_app with "Hpush1 [-]"). 
+      iApply (big_sepL2_app with "Hpush2 [-]").
+      iApply (big_sepL2_app with "Hpush3 [-]").
+      iApply (big_sepL2_app with "Hscall [-]").
+      iFrame. 
+    }
+    (* Next we close the adversary stack region so that it is Temporary *)
+    iMod (monotone_revoked_close_sub' _ (region_addrs s_first' e_r) RWLX (λ Wv, interp Wv.1 Wv.2)
+            with "[$Hsts $Hr Hstack_adv]") as "[Hsts Hex]".
+    { rewrite Hstackeq app_assoc. iDestruct (big_sepL_app with "Hstack_val") as "[_ Hstack_val']".
+      iApply big_sepL_sep. iSplitL.
+      - iDestruct (region_addrs_zeroes_trans with "Hstack_adv") as "Hstack_adv".
+        iApply (big_sepL_mono with "Hstack_adv"). iIntros (k y Hsome) "Hy".
+        iExists (inl 0%Z). iSplitR;auto. iFrame. simpl. iSplit.
+        + iAlways. iIntros (W1 W2 Hrelated12) "HW1 /=". by repeat (rewrite fixpoint_interp1_eq /=).
+        + by repeat (rewrite fixpoint_interp1_eq /=).
+      - iApply big_sepL_sep; iFrame "#". iApply big_sepL_forall. iPureIntro.
+        rewrite Hstackeq app_assoc in Hrevoked. apply Forall_app in Hrevoked as [_ Hrevoked]. 
+        intros k x Hsome. apply (Forall_lookup_1 _ _ k _ Hrevoked Hsome). 
+    }
+    (* We put the local stack in a non atomic invariant. Since the local stack will change, 
+       we allocate an STS to model that change *)
+    iMod (sts_alloc_loc _ (First : local_state) local_rel_pub local_rel_pub with "Hsts")
+      as (j) "(Hsts & % & % & Hstate & #Hrelj)".
+    iMod (na_inv_alloc logrel_nais ⊤ (regN.@"stack") (∃ x:local_state, sts_state_loc j First
+                       ∗ match x with
+                         | First => b_r ↦ₐ[RWLX] inr (RWX, Global, d, d, d)
+                                  ∗ a2 ↦ₐ[RWLX] inr (pc_p, pc_g, pc_b, pc_e, a_first)
+                                  ∗ a3 ↦ₐ[RWLX] inr (E, Global, b, e, a)
+                                  ∗ [[stack_own_b,s_last']]↦ₐ[RWLX][[ [inl w_1; inl w_2; inl w_3; inl w_4a; inl w_4b; inl w_4c; inr (pc_p, pc_g, pc_b, pc_e, rest0_first);
+                                                                       inr (RWLX, Local, b_r, e_r, s_last')] ]]
+                         | Second => True
+                         | Released => emp
+                         end 
+                       )%I
+            with "[Hstack_own Hstate Hb_r Ha2 Ha3]")
+      as "#Hlocal".
+    { iNext. iExists (First : local_state). iFrame "Hstate". 
+      iExact "Hstate". iFrame "Hstate".  }
+    
 End awkward_example. 
